progs/list.v
@@ -179,7 +179,18 @@ unfold ptr_neq; intros.
 rewrite lseg_unfold at 1; auto.
 destruct l.
 apply pred_ext; normalize.
-intros ? ? ? [? [? ?]]. inv H2.
+intros; discriminate.
+apply pred_ext; normalize.
+intro.
+apply exp_right with v; normalize.
+apply exp_right with l; normalize.
+apply exp_right with x0; normalize.
+apply andp_right; auto.
+rewrite (field_mapsto_typecheck_val list_struct list_data Share.top x v 
+                        list_structid 
+                    (Fcons list_data list_dtype
+                        (Fcons list_link (Tcomp_ptr list_structid noattr)
+                           Fnil))  noattr); auto.
 assert (UNROLL: unroll_composite_fields list_structid list_struct
        (Fcons list_data list_dtype
           (Fcons list_link (Tcomp_ptr list_structid noattr) Fnil)) =
@@ -191,29 +202,23 @@ apply list_unroll_dtype.
 rewrite if_true by auto.
 f_equal.
 symmetry. apply list_type_is.
-destruct list_access_mode as [ch ACC].
-normalize.
-apply pred_ext; normalize.
-intro y.
-rename v into h.
-apply (exp_right h).
-apply (exp_right l).
-apply (exp_right y).
-apply sepcon_derives; auto.
-normalize.
-rewrite (field_mapsto_typecheck_val list_struct list_data Share.top x h) at 1 by reflexivity.
-rewrite (field_mapsto_typecheck_val list_struct list_link Share.top x y) at 1 by reflexivity.
 rewrite UNROLL.
-simpl.
+simpl type_of_field. rewrite if_true by auto.
+normalize.
+forget (field_mapsto Share.top list_struct list_data x v) as foo.
+rewrite (field_mapsto_typecheck_val list_struct list_link Share.top x x0
+                        list_structid 
+                    (Fcons list_data list_dtype
+                        (Fcons list_link (Tcomp_ptr list_structid noattr)
+                           Fnil))  noattr); auto.
+rewrite UNROLL. simpl type_of_field.
+rewrite if_false by apply list_data_not_link.
 rewrite if_true by auto.
-rewrite if_false by apply list_data_not_link. rewrite if_true by auto.
 normalize.
 (***)
 intros.
-destruct H2 as [? [? ?]].
-symmetry in H2; inv H2.
-rename x2 into y.
-apply (exp_right y).
+inv H2.
+apply exp_right with x2.
 normalize.
 Qed.
 
@@ -248,324 +253,3 @@ simpl.
 
 Abort.
 End TestCase.
-
-(*
-DONE TO HERE.
-The rest is old stuff from msl/examples/cont/lseg.v
-
- 
-
-Lemma lseg_neq: forall vl p q: valt, 
-     is_list_type (snd p) ->
-     snd p = snd q ->
-    ~ (ptr_eq (fst p) (fst q)) ->
-        lseg vl p q = EX h: val, EX vl': list valt, 
-                !! (vl = (h,snd p)::vl') && 
-              field_mapsto Share.top (deref v1) data h * 
-              next link Share.top v1 (tail,snd v1) * |> lseg t (tail, snd v1) v2
-
-next p y *  |> lseg y q.
-Proof.
- intros.
- apply pred_ext.
- rewrite lseg_unfold at 1.
- apply orp_left.
- apply andp_left2. apply exp_derives; intro y.
- apply sepcon_derives; auto.
- apply prop_andp_left; contradiction.
- rewrite (lseg_unfold p q). apply orp_right1.
- apply prop_andp_right; auto.
-Qed.
-
-Lemma lseg_eq: forall a, lseg a a = emp.
-Proof.
- intros. rewrite lseg_unfold.
- apply pred_ext.
- apply orp_left.
- apply prop_andp_left; congruence.
- apply prop_andp_left; auto.
- apply orp_right2. apply prop_andp_right; auto. 
-Qed.
-
-Lemma lseg_cons: (* U2 *)
- forall x y z, x<>z -> next x y * lseg y z |-- lseg x z.
-Proof.
- intros.
- pattern lseg at 1; rewrite lseg_unfold.
- apply orp_right1.
- apply prop_andp_right; auto.
- apply exp_right with y.
- apply sepcon_derives; auto.
- unfold lseg.
- apply now_later.
-Qed.
-
-Lemma lseg_neq_0:  forall y, lseg 0 y |-- !! (y=0).  (* W2 *)
-Proof.
-  intros. 
-  rewrite lseg_unfold.
- apply orp_left.
- apply andp_left2.
- apply exp_left; intro v.
- rewrite next_gt_0.
- rewrite sepcon_andp_prop1.
- apply prop_andp_left; intro. inv H.
- apply andp_left1.
- intros w ?; hnf in *; auto.
-Qed.
-
-Lemma next_lseg:  (* U1 *)
-  forall x y, x<>y ->  next x y |-- lseg x y.
-Proof.
-  intros.
-  rewrite <- (sepcon_emp (next x _)).
-  rewrite <- (lseg_eq y).
-  eapply derives_trans; [ apply lseg_cons | ]; auto.
-Qed.
-
-
-Lemma mapsto_conflict:
-   forall a b c, mapsto a b  *  mapsto a c |-- FF.
-  Proof.
-    intros. intros w  [w1 [w2 [? [? ?]]]]; hnf.
-    specialize (H0 a). specialize (H1 a).
-    rewrite if_true in * by auto.
-    apply (resource_at_join _ _ _ a) in H.
-    rewrite H0 in H; rewrite H1 in H; inv H.
-    pfullshare_join.
- Qed.
-
-Lemma next_conflict:  (*  W3 *)
-   forall x y y', next x y * next x y' |-- FF.
-Proof.
-  unfold next; intros.
-  eapply derives_trans; [ | apply (mapsto_conflict x y y')].
-  apply sepcon_derives; apply andp_left2; auto.
-Qed.
-
-Lemma not_prop_right: forall P (Q: Prop), (Q -> P |-- FF) -> P |-- !! (not Q).
- Proof. intros. intros w ? ?. specialize (H H1 w H0); auto. 
-  Qed.
-
- Lemma next_conflict_list: (* W4 *)
-     forall x y z, next x y * lseg z 0 |-- !!(x<>z).
- Proof.
-   intros.
-   unfold next.
-   rewrite lseg_unfold.
-  rewrite sepcon_comm.
-  rewrite distrib_orp_sepcon.
-  apply orp_left.
-  repeat rewrite sepcon_andp_prop1. 
-  apply andp_left2.
-  rewrite exp_sepcon1.
-  apply exp_left; intro v. 
-  rewrite sepcon_comm.
-  rewrite <- sepcon_assoc.
-  apply @derives_trans with (!! (x<>z) && TT * TT).
-  apply sepcon_derives; auto.
-  apply andp_right; auto. 
-  apply not_prop_right; intros; subst; apply next_conflict.
-  rewrite sepcon_andp_prop1.
-  apply andp_left1; auto.
-  rewrite sepcon_andp_prop1. rewrite emp_sepcon.
-  apply prop_andp_left; intro.
-  subst.
-  unfold next.
-  apply prop_andp_left; intro.
-  intros ? ?; hnf; omega.
-Qed.
-
-Lemma lseg_W5: forall x y z,   (* W5 *)
-    lseg x y * lseg x z |-- !!(x=y \/ x=z).
-Proof.
-  intros.
-  destruct (eq_dec x y).
-  apply prop_right; auto.
-  destruct (eq_dec x z).
-  apply prop_right; auto.
-  rewrite (lseg_neq x y); auto.
-  rewrite exp_sepcon1; apply exp_left; intro.
-  rewrite (lseg_neq x z); auto.
-  rewrite exp_sepcon2; apply exp_left; intro.
-  rewrite sepcon_assoc. 
-  rewrite <- (sepcon_assoc (|> _)).
-  rewrite (sepcon_comm (|> _)).
-  repeat rewrite <- sepcon_assoc. rewrite sepcon_assoc.
-  eapply derives_trans. apply sepcon_derives. apply next_conflict. apply derives_refl.
-  rewrite FF_sepcon. auto.
-Qed.
-
-(* This lemma is not currently used, 
-    but it might be useful in a different proof of lseg_cons_in_mapsto_context, etc. *)
-Lemma sepcon_andp_fash'1 {A}{JA: Join A}{PA: Perm_alg A}{agA: ageable A}{AgeA: Age_alg A}:  
-    forall (P: pred nat) (Q R : pred A),  fash' P && Q * R = fash' P && (Q * R).
- Proof.
-  intros. apply pred_ext; intros w ?.
-   destruct H as [w1 [w2 [? [? ?]]]].
-   destruct H0. split.
-   hnf in H0|-*. replace (level w) with (level w1); auto.
-   apply join_level in H; intuition.
-    exists w1; exists w2; split3; auto.
-   destruct H.
-   destruct H0 as [w1 [w2 [? [? ?]]]]; exists w1; exists w2; split3; auto.
-   split; auto.
-   hnf in H|-*. replace (level w1) with (level w); auto.
-   apply join_level in H0; intuition.
-Qed.
-
-Lemma lseg_cons_in_next_context:   (*  U4 *)
-    forall x y z v, lseg x y * next y z * next z v |-- lseg x z * next z v.
-Proof.
-  intros.
-  apply @derives_trans with ((lseg x y * next y z) && (ewand (next z v) TT) *  next z v).
-  intros w [w1 [w2 [? [ ? ?]]]]. exists w1; exists w2; split3; auto. split; auto.
-  exists w2; exists w; split3; auto.
-  apply sepcon_derives; auto.
-  generalize (goedel_loeb (ALL x:adr,  
-    lseg x y * next y z && ewand (next z v) TT >=> lseg x z) TT) ; intro.
-  spec H.
-  2:  intros w ?; apply (H (@level _ R.ag_rmap w) I x w (le_refl _)); auto.
-  clear.
-  apply allp_right; intro x.
-  apply subp_i1.
-  intros w [[_ ?] [? ?]].
-  rewrite lseg_unfold. left.
-  split.
-  do 3 red. intro; subst x.
-  clear - H0 H1.
-  destruct H1 as [w1 [w2 [? [? _]]]].
-  assert (app_pred (next z v * (lseg z y * next y z)) w2) by (do 2 eexists; split3; eauto).
-  rewrite <- sepcon_assoc in H2.
-  destruct H2 as [wa [wb [? [? ?]]]].
-  assert (app_pred (lseg z y * (next y z * next z v)) w2).
-  rewrite sepcon_comm.
-  rewrite sepcon_assoc.
-  exists wb; exists wa; split3; auto.
-  clear - H5.
-  rewrite (lseg_unfold z y) in H5.
-  rewrite distrib_orp_sepcon in H5.
-  destruct H5.
-  repeat rewrite sepcon_andp_prop1 in H.
-  destruct H as [_ H].
-  repeat rewrite exp_sepcon1 in H.
-  destruct H as [u ?].
-  rewrite (sepcon_comm (next z u)) in H.
-  rewrite sepcon_assoc in H.
-  rewrite sepcon_comm in H.
-  rewrite (sepcon_comm (next y z)) in H.
-  rewrite <- sepcon_assoc in H.
-  rewrite sepcon_assoc in H.
-  destruct H as [w1 [w3 [? [? _]]]].
-  apply next_conflict in H0; auto.
-  rewrite sepcon_andp_prop1 in H. rewrite emp_sepcon in H.
-  destruct H. hnf in H. subst y.
-  apply next_conflict in H0; auto.
-  rewrite lseg_unfold in H0.
-  rewrite distrib_orp_sepcon in H0.
-  destruct H0.
-  repeat rewrite sepcon_andp_prop1 in H0.
-  destruct H0.
-  repeat rewrite exp_sepcon1 in H2.
-  destruct H2 as [u H2].
-  do 3 red in H0. exists u.
- rewrite later_allp in H.
-  specialize (H u).
-  rewrite sepcon_assoc in H2.
-  destruct H2 as [w1 [w2 [? [? ?]]]].
-  red in H. rewrite subp_later in H.
-  specialize (H w2).
-  spec H. apply join_level in H2; destruct H2; omega.
-  exists w1; exists w2; split3; auto.
-  apply H; auto.
-  rewrite later_andp. split.
-  rewrite later_sepcon.
-  eapply sepcon_derives; try apply H4; auto.
-  apply now_later.
-  eapply now_later; eauto.
-  clear - H2 H1.
-  destruct H1 as [w3 [w4 [? [? _]]]].
-  destruct (join_assoc H2 (join_comm H)) as [f [? ?]].
-  exists w3; exists f; split3; auto.
-  exists z.
-  rewrite lseg_eq.
-  rewrite sepcon_andp_prop1 in H0.
-  destruct H0. hnf in H0; subst y.
-  rewrite sepcon_comm in H2.
-  eapply sepcon_derives; try apply H2; auto.
-  apply now_later.
-Qed.
-
-Lemma list_append:  (* U3 *)
-   forall x y, lseg x y * lseg y 0 |-- lseg x 0.
-Proof.
- intros.
-  generalize (goedel_loeb (ALL x:adr, lseg x y * lseg y 0  >=> lseg x 0) TT) ; intro.
-  spec H; [ clear  | intros w ?; apply (H (@level _ R.ag_rmap w) I x w (le_refl _)); auto].
-  apply andp_left2.
-  apply allp_right; intro x.
-  apply subp_i1.
-  intros w [? ?].
-  destruct (eq_dec x 0).
-  subst. rewrite lseg_eq.
-  rewrite lseg_unfold in H0.
-  rewrite distrib_orp_sepcon in H0.
-  destruct H0.
-  rewrite sepcon_andp_prop1 in H0. destruct H0.
-  rewrite exp_sepcon1 in H1.
-  destruct H1 as [u ?]. unfold next in H1.
-  repeat rewrite sepcon_andp_prop1 in H1.
-  destruct H1 as [H1 _]; hnf in H1. inv H1. 
-  rewrite sepcon_andp_prop1 in H0. destruct H0. hnf in H0. subst.
-  rewrite lseg_eq in H1. rewrite sepcon_emp in H1. auto.
-  rewrite (lseg_unfold x y) in H0.
-  rewrite distrib_orp_sepcon in H0.
-  destruct H0.
-  rewrite sepcon_andp_prop1 in H0. destruct H0.
-  rewrite exp_sepcon1 in H1.
-  destruct H1 as [z H1].
-  rewrite lseg_neq; auto.
-  exists z.
-  rewrite sepcon_assoc in H1.
-  rewrite later_allp in H.
-  specialize (H z).
-  destruct H1 as [w1 [w2 [? [? ?]]]].
-  red in H. rewrite subp_later in H.
-  specialize (H w2).
-  spec H. apply join_level in H1; destruct H1; omega.
-  exists w1; exists w2; split3; auto.
-  apply H; auto.
-  rewrite later_sepcon.
-  eapply sepcon_derives; try apply H3; auto.
-  apply now_later.
-  rewrite sepcon_andp_prop1 in H0.
-  destruct H0. hnf in H0; subst y. rewrite emp_sepcon in H1; auto.
-Qed.
-
-Lemma lseg_U5:
-    forall x y z w, z<>w -> lseg x y * next y z * lseg z w |-- lseg x z * lseg z w.
-Proof.
- intros.
- rewrite (lseg_neq z w); auto.
- repeat rewrite exp_sepcon2.
- apply exp_derives; intro v.
- repeat rewrite <- sepcon_assoc.
- apply sepcon_derives; auto.
- apply lseg_cons_in_next_context.
-Qed.
-
-Lemma lseg_cons_in_list_context: 
-    forall x y z, lseg x y * next y z * lseg z 0 |-- lseg x z * lseg z 0.
-Proof.
-  intros.
-  destruct (eq_dec z 0).
-  subst. rewrite lseg_eq. repeat  rewrite sepcon_emp. 
-  eapply derives_trans; try apply list_append.
-  apply sepcon_derives; eauto.
-  rewrite next_gt_0.
-  apply prop_andp_left; intro.
-  apply next_lseg; omega.
-  apply lseg_U5; auto.
-Qed.
-
-*)
